
\documentclass[12pt]{article}
\usepackage{amsmath}
\usepackage{amssymb}
\usepackage{amsthm}

\newtheorem{definition}{Definition} %might need to adjust/delete this later%

\newcommand{\dn}{\ensuremath{\stackrel{\mbox{\scriptsize def}}{=}}}

\newcommand{\ZERO}{\textbf{0}}   
\newcommand{\ONE}{\textbf{1}}    

\newcommand{\der}{\textit{der}}
\newcommand{\shift}{\textit{shift}}
\newcommand{\shifts}{\textit{shifts}}

\newcommand{\fuse}{\textit{fuse}}
\newcommand{\mkeps}{\textit{mkeps}}
\newcommand{\intern}{\textit{intern}}

\newcommand{\Seq}{\textit{Seq}}
\newcommand{\Left}{\textit{Left}}
\newcommand{\Right}{\textit{Right}}
\newcommand{\Star}{\textit{Star}}
\newcommand{\Empty}{\textit{Empty}}

\newcommand{\Marked}[1]{\bullet\,#1}

\newcommand{\fin}{\textit{fin}}
\newcommand{\nullable}{\textit{nullable}}

\newcommand{\Bits}{\textit{Bits}}
\newcommand{\POINT}{\textit{POINT}}
\newcommand{\mkfin}{\textit{mkfin}}


\newcommand{\STARText}{\textit{Star} $(r^*)$}
\newcommand{\SEQText}{ \textit{Sequence} $(r_1 \cdot r_2)$}

\newcommand{\emptylist}{[\,]}

\newcommand{\At}{$\,@\,$}

\newcommand{\matcher}{\textit{matcher}}




\title{Shifts Proof}
%\author{Meshal Binnasban}
\date{\today}

\begin{document}

\maketitle

We consider two main cases, namely $shifts(ms,r)= []$ and $shifts(ms,r)\neq []$.
\section{Case 1: $shifts(ms,r) = []$}


We want to prove
\[
Strips(L(r^n))(set\,ms) = \varnothing.
\]

From the induction hypothesis 
\[
set(shifts(ms,r)) = Strips(L(r))(set\,ms).
\]

By assumption
\[
set(shifts(ms,r)) = \varnothing,
\]

so
\[
Strips(L(r))(set\,ms) = \varnothing.
\]

\subsection{sub case $nullable(r)$}
unfolding the shifts definition,
\[
set(shifts(ms,r^n)) = set(shifts(ms,r)) \cup set(shifts(shifts(ms,r),r^{n-1})),
\]
\[
= Strips(L(r))(set\,ms) \cup Strips(L(r^{n-1}))(Strips(L(r))(set\,ms)),
\]
\[
= \varnothing \cup Strips(L(r^{n-1}))(\varnothing) = \varnothing.
\]

\subsection{sub case $\neg nullable(r)$}
again, unfolding the shifts definition,

\[
set(shifts(ms,r^n)) = set(shifts(shifts(ms,r),r^{n-1})),
\]
\[
= Strips(L(r^{n-1}))(set(shifts(ms,r))),
\]
\[
= Strips(L(r^{n-1}))(\varnothing) = \varnothing.
\]

Therefore
\[
Strips(L(r^n))(set\,ms) = \varnothing.
\]

\newpage

\section{Case 2: $shifts(ms,r) \neq []$}

We want to prove
\[
set(shifts(ms,r^n)) = Strips(L(r^n))(set\,ms).
\]

\subsection{sub case $nullable(r)$}

unfolding the shifts definition,
\[
set(shifts(ms,r^n)) = a \cup b,
\]
\[
a := set(shifts(ms,r)), \quad b := set(shifts(shifts(ms,r), r^{n-1})).
\]

by IH on $P(ms,r)$,
\[
a = Strips(L(r))(set\,ms).
\]

since $shifts(ms,r)$ is smaller than $ms$ and $r^{n-1}$ is smaller than $r^{n}$, we can use IH on $P(shifts(ms,r), r^{n-1})$,
\[
b = Strips(L(r^{n-1}))(set(shifts(ms,r))) = Strips(L(r^{n-1}))(Strips(L(r))(set\,ms)).
\]

therefore
\[
set(shifts(ms,r^n)) = a \cup b
= Strips(L(r))(set\,ms) \cup Strips(L(r^{n-1}))(Strips(L(r))(set\,ms)).
\]

by Strips properties:
with nullable A, and B
 \[Strips (A\,@\, B) C= (Strips\, B\, (Strips\, A\, C)) \cup Strips\, A\,C \cup Strips\, B\, C\]
\[A=L(r) \texttt{ and } B=L(r^{n-1})  \]
\[L{r^n} = L(r)\, @\, L(r^{n-1})\]
we have $Strips\, B\, (Strips\, A\, C) = Strips(L(r^{n-1}))(Strips(L(r))(set\,ms))$
and $Strips\, A\,C =Strips(L(r))(set\,ms)$

but missing the third $Strips\, B\,C =Strips(L(r^{n-1}))(set\,ms)$


\subsection{sub case $\neg nullable(r)$}

unfolding the shifts definition,
\[
set(shifts(ms,r^n)) = b,
\]
\[
b := set(shifts(shifts(ms,r), r^{n-1})).
\]

since $shifts(ms,r)$ is smaller than $ms$ and $r^{n-1}$ is smaller than $r^{n}$, we can use IH on $P(shifts(ms,r), r^{n-1})$,
\[
b = Strips(L(r^{n-1}))(set(shifts(ms,r))) = Strips(L(r^{n-1}))(Strips(L(r))(set\,ms)).
\]

by Strips properties:
with not nullable A, and B
 \[Strips (A\,@\, B) C= Strips\, B\, (Strips\, A\, C)\]
\[A=L(r) \texttt{ and } B=L(r^{n-1})  \]
\[L{r^n} = L(r)\, @\, L(r^{n-1})\]
therefore
\[ set(shifts(ms,r^n)) = Strips(L(r^n))(set\, ms)\]


\newpage
\section{notes}
\subsection{case 1}
i thought i would start with two cases to consider, namely $shifts(ms, r) = []$ 
and $shifts(ms, r) \neq []$. similar to the urlues. 

i started with first one. so first, i assumed that $shifts(ms, r) = []$ and need to prove $Strips(r^n)(set ms) = \varnothing$.

since $r$ is smaller, we can use $p(ms,r^n)$ so 

$set(shifts (ms r)) = Strips (L r )(set ms)$. 

by assumption, lhs is $\varnothing$ so now we have $Strips (L r)(set ms) = \varnothing$.

now we need to prove $Strips( L r^n)(set ms) = \varnothing$.
again two cases to consider, 1- nullable $r$.

unfolding shifts definition. 
\[set ( shifts r^n ms)= set(shifts r ms) U set (shifts (shifts ms r) r^n-1)\]

that equals to $Strip( L r )(set ms) U Strips( L r^n-1)(Strips L r ) (set ms)$. 

the lhs of union =$\varnothing$ 

and rhs= $Strips( L r^n-1) \varnothing (set ms) = \varnothing$. 

in the second case where $r$ is not nullable: 

unfolding shifts again:

\[set ( shifts r^n ms) = set ( shifts r^{n-1} (shifts r ms) ) = Strip( r^{n-1})(Strip(L r ms))\]
 
and since $Strip(L r ms)=\varnothing$ so it becomes $Strip( r^n-1) \varnothing$ and so = $\varnothing$.
\subsection{case 2}
NTIMES:
for the second case, i assume $shifts(ms, r) \neq []$. i need to prove $set(shifts(ms,r^n)) = Strips(L\,r^n)(set\,ms)$. again two cases to consider, 1- nullable $r$.

unfolding shifts definition,  
$set(shifts(ms,r^n)) = a \cup b$  
where  
$a = set(shifts(ms,r))$  
$b = set(shifts(shifts(ms,r), r^{n-1}))$

for $a$, use IH $P(ms,r)$ to get  
$a = Strips(L\,r)(set\,ms)$

for $b$, we can use IH $P(shifts(ms,r), r^{n-1})$ since (i) $shifts(ms,r)$ is smaller than $ms$ and (ii) $r^{n-1}$ is smaller than $r^{n}$. hence  
$b = Strips(L\,r^{n-1})(set(shifts(ms,r))) = Strips(L\,r^{n-1})(Strips(L\,r)(set\,ms))$

therefore  
$set(shifts(ms,r^n)) = a \cup b = Strips(L\,r)(set\,ms) \cup Strips(L\,r^{n-1})(Strips(L\,r)(set\,ms))$

in the second case where $r$ is not nullable:

unfolding shifts again,  
$set(shifts(ms,r^n)) = b$  
where  
$b = set(shifts(shifts(ms,r), r^{n-1})) = Strips(L\,r^{n-1})(set(shifts(ms,r))) = Strips(L\,r^{n-1})(Strips(L\,r)(set\,ms))$

and since $L(r^n) = L(r)@L(r^{n-1})$ we have  
$b = Strips(L\,r @ L\,r^{n-1})(set\,ms) = Strips(L\,r^n)(set\,ms)$


\bibliographystyle{abbrv}
\bibliography{urules}
\addcontentsline{toc}{section}{References}


\end{document}